\documentclass[a4paper,11pt]{article}
\usepackage[T1]{fontenc}
\usepackage[utf8]{inputenc}
\usepackage{lmodern}
\usepackage{amsmath}
\usepackage{amsfonts}

\usepackage{graphicx}

\title{Assignment \#2 -- Introduction to Robotics}
\author{
Luisa Zintgraf \texttt{6027303} \\
Weipeng He \texttt{6411529} \\
Philipp Ruppel \texttt{6248024}
}

\begin{document}

\maketitle

\section{}
\subsection{}
For each joint, the transformation is:
\[
  ^{i-1}A_{i} = 
  \begin{pmatrix}
    C_i & -S_i & 0 & a_iC_i \\
    S_i & C_i & 0 & a_iS_i \\
    0 & 0 & 1 & 0 \\
    0 & 0 & 0 & 1
  \end{pmatrix}
\]
where $C_i = cos(\theta_i)$ and $S_i = sin(\theta_i)$.

\begin{align*}
  ^{0}A_{1} {}^{1}A_{2} {}^{2}A_{3} &= 
  \begin{pmatrix}
    C_1C_2 - S_1S_2 & -S_1C_2 - C_1S_2 & 0 & a_2C_1C_2 - a_2S_1S_2 + a_1C_1 \\
    C_1S_2 + S_1C_2 & -S_1S_2 + C_1C_2 & 0 & a_2S_1C_2 + a_2C_1S_2 + a_1S_1 \\
    0 & 0 & 1 & 0 \\
    0 & 0 & 0 & 1
  \end{pmatrix}
  {}^{2}A_{3} \\
  &= 
  \begin{pmatrix}
    C_{1+2} & -S_{1+2} & 0 & a_1C_1 + a_2C_{1+2} \\
    S_{1+2} & C_{1+2} & 0 & a_1S_1 + a_2S_{1+2} \\
    0 & 0 & 1 & 0 \\
    0 & 0 & 0 & 1
  \end{pmatrix}
  {}^{2}A_{3}  \\
  &= 
  \begin{pmatrix}
    C_{1+2+3} & -S_{1+2+3} & 0 & a_1C_1 + a_2C_{1+2} + a_3C_{1+2+3} \\
    S_{1+2+3} & C_{1+2+3} & 0 & a_1S_1 + a_2S_{1+2} + a_3S_{1+2+3} \\
    0 & 0 & 1 & 0 \\
    0 & 0 & 0 & 1
  \end{pmatrix}
\end{align*}
where $C_{1+2} = cos(\theta_1 + \theta_2)$, $C_{1+2+3} = cos(\theta_1 + \theta_2 + \theta_3)$, $S_{1+2} = sin(\theta_1 + \theta_2)$ and $S_{1+2+3} = sin(\theta_1 + \theta_2 + \theta_3)$. 

We have $\theta_1 + \theta_2 + \theta_3 = \pi$, therefore $C_{1+2+3} = -1$, $S_{1+2+3} = 0$, $C_{1+2} = -C_3$ and $S_{1+2} = S_3$. Thus,
\[
  ^0T_3 = {}^{0}A_{1} {}^{1}A_{2} {}^{2}A_{3} =
  \begin{pmatrix}
    -1 & 0 & 0 & a_1C_1 - a_2C_3 - a_3 \\
    0 & -1 & 0 & a_1S_1 + a_2S_3 \\
    0 & 0 & 1 & 0 \\
    0 & 0 & 0 & 1
  \end{pmatrix}
\]

\subsection{}
We have the homogeneous tranformations as they are said.
\[
  {}^{-1}A_{0} = 
  \begin{pmatrix}
    1 & 0 & 0 & 0 \\
    0 & C_0 & -S_0 & 0 \\
    0 & S_0 & C_0 & 0 \\
    0 & 0 & 0 & 1
  \end{pmatrix}
\]
and
\[
  {}^{3}A_{4} = 
  \begin{pmatrix}
    1 & 0 & 0 & 0 \\
    0 & C_4 & -S_4 & 0 \\
    0 & S_4 & C_4 & 0 \\
    0 & 0 & 0 & 1
  \end{pmatrix}
\]

Then, the whole transformation will be:
\[
  T = {}^{-1}A_{0} {}^{0}A_{1} {}^{1}A_{2} {}^{2}A_{3} {}^{3}A_{4}
\]

\end{document}
